Play with tailrec

CFGraph/Eval.thy
@@ -23,28 +23,27 @@ fun evalV :: "val \<Rightarrow> benv \<Rightarrow> venv \<Rightarrow> d"
               Some l \<Rightarrow> (case ve (var,l) of Some d \<Rightarrow> d))"
   |     "evalV (L lam) \<beta> ve = DC (lam, \<beta>)"
 
-function (sequential,domintros)
+function (sequential,domintros,tailrec)
          evalF :: "d \<Rightarrow> (d list) \<Rightarrow> venv \<Rightarrow> contour \<Rightarrow> ans"
      and evalC :: "call \<Rightarrow> benv \<Rightarrow> venv \<Rightarrow> contour \<Rightarrow> ans"
   where "evalF (DC (Lambda lab vs c, \<beta>)) as ve b
-          = (case length vs = length as of True \<Rightarrow>
-            let \<beta>' = \<beta> (lab \<mapsto> b);
-                ve' = map_upds ve (map (\<lambda>v.(v,b)) vs) as
-            in evalC c \<beta>' ve' b
+          = (if length vs = length as
+             then let \<beta>' = \<beta> (lab \<mapsto> b);
+                      ve' = map_upds ve (map (\<lambda>v.(v,b)) vs) as
+                  in evalC c \<beta>' ve' b
+             else undefined
             )"
   |     "evalF (DP (Plus c)) as ve b 
-          = (case as of
-               [DI a1, DI a2, cont] \<Rightarrow> 
+          = (case as of [DI a1, DI a2, cont] \<Rightarrow> 
                   (let b' = Suc b
                    in evalF cont [DI (a1 + a2)] ve b'))"
   |     "evalF (DP (If ct cf)) as ve b
-          = (case as of
-               [DI v, contt, contf] \<Rightarrow> (      
+          = (case as of [DI v, contt, contf] \<Rightarrow> (      
                   let b' = Suc b
                    in if v \<noteq> 0 then evalF contt [] ve b'
                                else evalF contt [] ve b'))"
-  |     "evalF Stop as _ _ = (
-                case as of [DI i] \<Rightarrow> i)"
+  |     "evalF Stop as _ _
+          = (case as of [DI i] \<Rightarrow> i)"
 
   |     "evalC (App lab f vs) \<beta> ve b
           = (let f' = evalV f \<beta> ve;
@@ -56,8 +55,43 @@ function (sequential,domintros)
                  \<beta>' = \<beta> (lab \<mapsto> b');
                  ve' = ve ++ map_of (map (\<lambda>(v,l). ((v,b'), evalV (L l) \<beta>' ve)) ls)
             in evalC c' \<beta>' ve' b')"
-  by pat_completeness auto
+  apply pat_completeness
+  apply auto
+done
 
 print_theorems
 
-end
+thm evalF_evalC.domintros(1)
+
+definition evalCPS :: "prog \<Rightarrow> int"
+  where "evalCPS l = (let ve = empty;
+                          \<beta> = empty;
+                          f = evalV (L l) \<beta> ve
+                      in  evalF f [Stop] ve 0)"
+
+definition eval_terminates :: "prog \<Rightarrow> bool" where
+    "eval_terminates l = (
+       let ve = empty;
+           \<beta> = empty;
+           f = evalV (L l) \<beta> ve
+       in evalF_evalC_dom (Inl (f, [Stop], ve, 0)))"
+
+lemma ex1_terminates[simp]: "eval_terminates ex1"
+unfolding eval_terminates_def
+by (auto intro!:evalF_evalC.domintros)
+
+lemma ex1_correct: "evalCPS ex1 = 0"
+unfolding evalCPS_def
+apply simp
+apply (insert ex1_terminates)
+unfolding eval_terminates_def
+apply simp
+thm evalF_evalC.domintros(1)
+thm evalC.psimps(1)
+apply (erule evalC.psimps(1))
+
+apply (auto intro!:evalF_evalC.domintros)
+
+apply simp
+
+apply
